proofs/transform/eliminate_algebraic_proofs/eliminate_algebraic_semantics.v
@@ -178,6 +178,331 @@ Proof.
   destruct (match_val_single g2_valid pd pdf2 vt _ p1 (Forall_inv Hpats2) d ) eqn : Hmatch1; auto.
 Qed.
 
+Lemma in_split_nodup {A B: Type} {f: A -> B} {x: A} {l: list A}
+  (Hn: NoDup (map f l))
+  (Hin: In x l):
+  exists l1 l2: list A, l = l1 ++ x :: l2 /\ forall y, In y l1 \/ In y l2 -> f y <> f x.
+Proof.
+  destruct (in_split _ _ Hin) as [l1 [l2 Hl]]. subst.
+  exists l1. exists l2. split; auto.
+  intros y Hiny.
+  rewrite map_app in Hn. simpl in Hn.
+  rewrite NoDup_app_iff' in Hn.
+  destruct Hn as [_ [Hn Hnotin]].
+  destruct Hiny as [Hiny | Hiny].
+  - intros Hfeq. apply (Hnotin (f x)). simpl. split; auto.
+    rewrite in_map_iff. exists y; auto.
+  - clear Hnotin. inversion Hn as [| ? ? Hnotin ?]; subst.
+    intros Hfeq. apply Hnotin. rewrite in_map_iff. exists y; auto.
+Qed.
+  
+
+Lemma match_rep_simple_constr {gamma} (gamma_valid: valid_context gamma) {m a c}
+  (m_in: mut_in_ctx m gamma) (a_in: adt_in_mut a m) (c_in: constr_in_adt c a) {args}
+  (args_length: length args = length (m_params m))
+  {pd pdf} pf vt vv (b1: bool) {ty} {ps} d 
+  (Hty1: Forall (fun x : pattern * gen_term b1 => pattern_has_type gamma (fst x) (vty_cons (adt_name a) args)) ps) 
+  (Hty2: Forall (fun x : pattern * gen_term b1 => gen_typed gamma b1 (snd x) ty) ps) 
+  (Hsimp: simple_pat_match (map fst ps))
+  {tys vars t2} (Hinc: In (Pconstr c tys (map Pvar vars), t2) ps)
+  {al: arg_list (domain (dom_aux pd)) (sym_sigma_args c (map (v_subst vt) args))}
+  (Hsem: semantic_constr gamma_valid pd pdf vt m_in a_in c_in args_length d al):
+  match_rep gamma_valid pd pdf vt vv (term_rep gamma_valid pd pdf vt pf) (formula_rep gamma_valid pd pdf vt pf)
+    b1 ty (vty_cons (adt_name a) args) d ps Hty1 Hty2 =
+  (gen_rep gamma_valid pd pdf pf vt (val_with_args pd vt vv vars al) ty t2 (Forall_In Hty2 Hinc)).
+Proof.
+  (*Idea: use NoDups from simple pattern, split, use fact that we have vars - probably
+    simplify [matches_row] even further (can assume variable tbh)*)
+  assert (Hsimp1:=Hsimp). apply simple_pat_match_structure in Hsimp1.
+  destruct Hsimp1 as [b [cs [Hnotnull [Hnodup Hps]]]].
+  (* pose proof (combine_eq ps) as Hcomb. *)
+  apply map_eq_app in Hps.
+  destruct Hps as [ps1 [ps2 [Hps [Hmap1 Hmap2]]]].
+  subst.
+  (*Now need to split further: before c and after c*)
+  assert (Hin:=Hinc).
+  rewrite in_app_iff in Hin.
+  destruct Hin as [Hin | Hin].
+  2: { apply (in_map fst) in Hin. rewrite Hmap2 in Hin. destruct b; [|contradiction].
+    destruct Hin as [Heq1 | []]; discriminate.
+  }
+  assert (Hin':=Hin).
+  apply (in_map fst) in Hin. rewrite Hmap1 in Hin.
+  simpl in Hin. rewrite in_map_iff in Hin. destruct Hin as [[[c1 tys1] vs1] [Hpeq Hinx]].
+  simpl in Hpeq. inversion Hpeq; subst.
+  destruct (in_split_nodup Hnodup Hinx) as [cs1 [cs2 [Hcs Huniq]]].
+  simpl in Huniq.
+  subst cs. (*Now split ps correspondingly*)
+  rewrite map_app in Hmap1.
+  apply map_eq_app in Hmap1.
+  destruct Hmap1 as [psa [psb [Hps1 [Hmapa Hmapb]]]].
+  subst ps1.
+  simpl in Hmapb. destruct psb as [| [p3 t3] psb]; [discriminate|].
+  simpl in Hmapb. injection Hmapb. clear Hmapb. intros Hmapb Hp3; subst p3.
+  (*Tricky: nodups is according to map fst, but need snd for terms*)
+  assert (Ht3: t3 = t2 /\ vars = vs1). {
+    rewrite in_app_iff in Hin'. destruct Hin' as [Hin' | Hin'].
+    - (*Cannot be in psa by nodup*)
+      apply (in_map fst) in Hin'. rewrite Hmapa in Hin'.
+      rewrite in_map_iff in Hin'. destruct Hin' as [x [Heq1 Hinx']].
+      inversion Heq1; subst. specialize (Huniq x). forward Huniq; auto. contradiction.
+    - simpl in Hin'. (*In this case, good*) destruct Hin' as [Hin' | Hin'].
+      { inversion Hin'; subst. split; auto. apply (map_inj Pvar); auto. intros x y Hxy. inversion Hxy; auto. } 
+      (*Otherwise, same in psb*)
+      apply (in_map fst) in Hin'. rewrite Hmapb in Hin'.
+      rewrite in_map_iff in Hin'. destruct Hin' as [x [Heq1 Hinx']].
+      inversion Heq1; subst. specialize (Huniq x). forward Huniq; auto. contradiction.
+  }
+  destruct Ht3; subst t3 vs1.
+  (*Now reason about pattern match*) 
+  generalize dependent (Forall_In Hty2 Hinc). clear Hinc. 
+  revert Hty1 Hty2. rewrite <- app_assoc. intros Hty1 Hty2 Hty.
+  rewrite match_rep_app2.
+  2: {
+    (*Prove constr not in list*)
+    intros [p t] Hp Hinps1.
+    apply (in_map fst) in Hinps1.
+    rewrite Hmapa in Hinps1.
+    rewrite in_map_iff in Hinps1. destruct Hinps1 as [[[c2 tys2] vs2] [Hpeq2 Hinx2]].
+    simpl in Hpeq2. subst p. simpl in Hp.
+    simpl fst. eapply match_val_single_constr_nomatch; eauto.
+    specialize (Huniq (c2, tys2, vs2) (ltac:(auto))). auto.
+  }
+  (*Now simplify to [match_val_constr]*)
+  Opaque match_val_single. simpl.
+  (*Use result about [match_val_single] for semantic_constr*)
+  assert (Hpty: pattern_has_type gamma (Pconstr c tys (map Pvar vars)) (vty_cons (adt_name a) args)). {
+    rewrite Forall_forall in Hty1. apply (Hty1 (Pconstr c tys (map Pvar vars), t2)).
+    rewrite in_app_iff. simpl; auto.
+  }
+  assert (Htys: tys = args). {
+    eapply constr_pattern_is_constr in Hpty; eauto. destruct_all; auto.
+  }
+  subst tys.
+  assert (Hrow: @row_typed gamma (ty_subst_list (s_params c) args (s_args c)) (map Pvar vars)) by
+    (apply constr_typed_row in Hpty; auto).
+  assert (Heq: sym_sigma_args c (map (v_subst vt) args) =
+    map (v_subst vt) (ty_subst_list (s_params c) args (s_args c))).
+  {
+    apply sym_sigma_args_map. rewrite (adt_constr_params gamma_valid m_in a_in c_in); auto.
+  }
+  erewrite match_val_single_constr_row with (Hrow:=Hrow)(Heq:=Heq); eauto.
+  (*Now simplify [matches_row] *)
+  destruct (matches_row_allvars gamma_valid pd pdf vt vv _ _ Heq al vars Hrow) as [l [Hroweq Hl]].
+  rewrite Hroweq.
+  destruct b1; simpl; [erewrite term_rep_irrel | erewrite fmla_rep_irrel];
+  [apply tm_change_vv|apply fmla_change_vv]; auto.
+Qed.
+
+Check substi_mult.
+(*NOTE: what is the difference between [substi_mult] and [val_with_args]? Are they redundant?*)
+(*Yes, this lemma shows that they are the same. oops (TODO: remove one)*)
+Lemma substi_mult_val_with_args pd vt vv vs al x:
+  NoDup vs ->
+  substi_mult pd vt vv vs al x = val_with_args pd vt vv vs al x.
+Proof.
+  intros Hn.
+  destruct (in_dec vsymbol_eq_dec x vs) as [Hin| Hnotin].
+  2: { rewrite substi_mult_notin; auto. rewrite val_with_args_notin; auto. }
+  destruct (In_nth _ _ vs_d Hin) as [i [Hi Hx]]; subst.
+  assert (Heq: nth i (map (v_subst vt) (map snd vs)) s_int = v_subst vt (snd (nth i vs vs_d))).
+  { rewrite map_map. rewrite map_nth_inbound with (d2:=vs_d); auto. }
+  rewrite val_with_args_in with (Heq:=Heq); auto; [|solve_len].
+  rewrite substi_mult_nth' with (Hi:=Hi); auto.
+  apply dom_cast_eq.
+Qed.
+
+(*TODO: is [substi_multi_let] the same?*)
+(*NOTE: we really need to consolidate these*)
+Lemma substi_mult_let_equiv {gamma} (gamma_valid: valid_context gamma) 
+  pd pdf pf vt (vv: val_vars pd vt) (vs: list (vsymbol * term))
+  (*(Hn: NoDup (map fst vs))*)
+  (Hall: Forall (fun x => term_has_type gamma (snd x) (snd (fst x))) vs)
+  (Hdisj: forall v t, In v (map fst vs) -> In t (map snd vs) -> ~ In v (tm_fv t))
+  (*TODO: replace*)
+  (Hall2: Forall2 (fun (t : term) (ty : vty) => term_has_type gamma t ty) (map snd vs) (map snd (map fst vs))) x:
+  substi_multi_let gamma_valid pd pdf vt pf vv vs Hall x =
+  substi_mult pd vt vv (map fst vs) (terms_to_hlist gamma_valid pd pdf pf vt vv (map snd vs) (map snd (map fst vs))
+    Hall2) x.
+Proof.
+  (*Have to prove by induction because we didn't prove anything about values of [substi_multi_let]*)
+  revert vv.
+  induction vs as [| [v1 t1] vs]; simpl; intros vv; auto.
+  simp terms_to_hlist. simpl in Hdisj. simpl.
+  rewrite term_rep_irrel with (Hty2:=(Forall2_inv_head Hall2)).
+  rewrite IHvs with (Hall2:=(Forall2_inv_tail Hall2)); auto. simpl.
+  (*Use disjointness result*)
+  erewrite terms_to_hlist_change_vv. reflexivity.
+  intros tm v Hintm Hinv. unfold substi.
+  destruct (vsymbol_eq_dec v v1); subst; auto.
+  exfalso. apply (Hdisj v1 tm); auto.
+Qed. 
+
+
+Lemma fold_let_rep {gamma} (gamma_valid: valid_context gamma) pd pdf pf vt vv
+  (l: list (term * vsymbol)) (t: term) ty (Hty: term_has_type gamma (fold_let Tlet l t) ty) 
+  (Hty1: term_has_type gamma t ty)
+  (Htys: Forall2 (term_has_type gamma) (map fst l) (map snd (map snd l)))
+  (Hn: NoDup (map snd l))
+  (Hdisj: forall v t, In v (map snd l) -> In t (map fst l) -> ~ In v (tm_fv t))
+  :
+  term_rep gamma_valid pd pdf vt pf vv (fold_let Tlet l t) ty Hty =
+  term_rep gamma_valid pd pdf vt pf (val_with_args pd vt vv (map snd l) 
+    (terms_to_hlist gamma_valid pd pdf pf vt vv (map fst l) _ Htys)) t ty Hty1.
+Proof.
+  (*Instead (for now), prove with [substi_multi_let]*)
+  symmetry.
+  rewrite tm_change_vv with (v2:=substi_mult pd vt vv (map snd l) 
+    (terms_to_hlist gamma_valid pd pdf pf vt vv (map fst l) _ Htys)).
+  2: { intros; symmetry; apply substi_mult_val_with_args; auto. }
+  assert (Hflip: Forall (fun x : string * vty * term => term_has_type gamma (snd x) (snd (fst x))) (flip l)).
+  { unfold flip. rewrite Forall_map. simpl.
+    clear -Htys. induction l as [| h t IH]; simpl; auto. inversion Htys; subst; auto.
+  }
+  rewrite tm_change_vv with (v2:=substi_multi_let gamma_valid pd pdf vt pf vv (flip l) Hflip).
+  - (*Now prove main claim*)
+    clear.
+    revert vv. revert Hflip Hty. induction l as [| [t1 v1] tl IH]; intros Hflip Hty vv; auto.
+    + simpl. apply term_rep_irrel.
+    + simpl. simpl_rep_full. 
+      rewrite IH with (Hty:=(proj2' (ty_let_inv Hty))); auto.
+      apply tm_change_vv. intros x Hinx. unfold substi.
+      destruct (vsymbol_eq_dec x v1); subst; auto. simpl.
+      apply term_rep_irrel.
+  - (*prove last equality*)
+    intros x Hinx.
+    assert (Hflip': Forall2 (fun (t0 : term) (ty0 : vty) => term_has_type gamma t0 ty0) (map snd (flip l))
+      (map snd (map fst (flip l)))).
+    { rewrite map_snd_flip, map_fst_flip. auto. } 
+    rewrite substi_mult_let_equiv with (Hall2:=Hflip').
+    + revert Hflip'. rewrite map_fst_flip, map_snd_flip. intros.
+      erewrite terms_to_hlist_irrel. reflexivity.
+    + rewrite map_fst_flip, map_snd_flip. auto.
+Qed.
+
+
+Lemma val_with_args_cast pd vt vv vs1 vs2 srts1 srts2 (Heqvs: vs1 = vs2) 
+  (Heq: srts1 = srts2) (al: arg_list (domain (dom_aux pd)) srts1):
+  val_with_args pd vt vv vs1 al =
+  val_with_args pd vt vv vs2 (cast_arg_list Heq al).
+Proof.
+  subst. reflexivity.
+Qed.
+
+Lemma constr_pattern_var_types {gamma} {m a c} (m_in: mut_in_ctx m gamma)
+  (a_in: adt_in_mut a m) (c_in: constr_in_adt c a) {args} (args_len: length args = length (m_params m))
+  {vars} (Hty: pattern_has_type gamma (Pconstr c args (map Pvar vars)) (vty_cons (adt_name a) args)) :
+  map snd vars = ty_subst_list (s_params c) args (s_args c).
+Proof.
+  inversion Hty; subst. unfold ty_subst_list.
+  apply list_eq_ext'; rewrite !map_length in *; auto.
+  intros n d Hn.
+  specialize (H9 (Pvar (nth n vars vs_d), ty_subst (s_params c) args (nth n (s_args c) d))).
+  forward H9.
+  { rewrite in_combine_iff; [|solve_len]. simpl_len. exists n. split; auto.
+    intros d1 d2. rewrite map_nth_inbound with (d2:=vs_d) by auto.
+    rewrite map_nth_inbound with (d2:=d) by (unfold vsymbol in *; lia).
+    reflexivity.
+  }
+  simpl in H9.
+  inversion H9; subst.
+  rewrite map_nth_inbound with (d2:=vs_d); auto.
+  rewrite map_nth_inbound with (d2:=d); auto.
+  unfold vsymbol in *; lia.
+Qed.
+
+(*TODO: move*)
+Check terms_to_hlist.
+
+Lemma tm_hlist_cast {tys i} vt (Hi: i < length tys): 
+  v_subst vt (nth i tys vty_int) = nth i (map (v_subst vt) tys) s_int.
+Proof.
+  rewrite map_nth_inbound with (d2:=vty_int); auto.
+Qed.
+
+Lemma tm_hlist_ty {gamma} {ts: list term} {tys: list vty}
+  (Htys: Forall2 (term_has_type gamma) ts tys) {i} (Hi: i < length tys):
+  term_has_type gamma (nth i ts tm_d) (nth i tys vty_int).
+Proof.
+  rewrite Forall2_nth in Htys. destruct Htys as [Hlen Hith].
+  apply Hith; lia.
+Qed.
+
+Lemma terms_to_hlist_hnth {gamma} (gamma_valid: valid_context gamma) pd pdf pf vt vv (ts: list term)
+  (tys: list vty) (Htys: Forall2 (term_has_type gamma) ts tys) (i: nat) (Hi: i < length tys):
+  hnth i (terms_to_hlist gamma_valid pd pdf pf vt vv ts tys Htys) s_int (dom_int _) =
+  dom_cast (dom_aux pd) (tm_hlist_cast vt Hi) 
+    (term_rep gamma_valid pd pdf vt pf vv (nth i ts tm_d) (nth i tys vty_int) (tm_hlist_ty Htys Hi)).
+Proof.
+  generalize dependent (tm_hlist_cast vt Hi).
+  generalize dependent (tm_hlist_ty Htys Hi).
+  generalize dependent i.
+  generalize dependent tys.
+  induction ts as [| thd ttl IH]; intros [| ty tyl] Htys i Hi Hty Heq; try solve[inversion Htys].
+  - simpl in Hi; lia.
+  - simpl in Hi. simpl. simp terms_to_hlist.
+    destruct i as [|i'].
+    + simpl. simpl in Heq. assert (Heq = eq_refl). apply UIP_dec, sort_eq_dec. subst.
+      unfold dom_cast; simpl. apply term_rep_irrel.
+    + simpl. apply IH. lia.
+Qed.
+
+Check find_constr_rep.
+Check tm_semantic_constr.
+Check find_tm_semantic_constr.
+(*Relate [tm_semantic_constr] and [find_constr_rep*)
+(* Lemma tm_semantic_constr_rep {gamma} (gamma_valid: valid_context gamma} {m a c}
+  (m_in: mut_in_ctx m gamma) (a_in: adt_in_mut a m) (c_in: constr_in_adt c a)
+
+
+find_constr_rep
+     : forall (gamma_valid : valid_context ?gamma) (m : mut_adt) (m_in : mut_in_ctx m ?gamma)
+         (srts : list sort) (srts_len : Datatypes.length srts = Datatypes.length (m_params m))
+         (domain_aux : sort -> Set) (t : alg_datatype) (t_in : adt_in_mut t m)
+         (dom_adts : forall a : alg_datatype,
+                     mut_in_ctx m ?gamma ->
+                     forall Hin : adt_in_mut a m,
+                     domain domain_aux (typesym_to_sort (adt_name a) srts) =
+                     adt_rep m srts domain_aux a Hin),
+       uniform m ->
+       forall x : adt_rep m srts domain_aux t t_in,
+       {f : funsym &
+       {Hf : constr_in_adt f t * arg_list (domain domain_aux) (sym_sigma_args f srts)
+       | x = constr_rep gamma_valid m m_in srts srts_len domain_aux t t_in f (fst Hf) dom_adts (snd Hf)}} *)
+
+Lemma scast_switch {A B C: Set} (H1: A = B) (H2: C = B) (x1: A) (x2: C):
+  scast H1 x1 = scast H2 x2 ->
+  x2 = scast (eq_trans H1 (eq_sym H2)) x1.
+Proof.
+  intros Hcast. subst. simpl in Hcast. subst. simpl. reflexivity.
+Qed.
+
+Ltac gen_dom_cast := repeat match goal with |- context [dom_cast ?pd ?Heq ?x] =>
+            let y := fresh "y" in
+            set (y := dom_cast pd Heq x) in *; 
+            generalize dependent Heq 
+          end; simpl.
+
+Lemma scast_eq_uip' {A1 A2 : Set} (H1 H2 : A1 = A2) (x y : A1):
+  x = y ->
+  scast H1 x = scast H2 y.
+Proof.
+  intros; subst. simpl. (*ugh Equations ruins this*)
+  assert (H2 = eq_refl) by (apply Cast.UIP). subst; reflexivity.
+Qed.
+
+(*TODO: move*)
+
+Lemma index_eq_nodup {A: Type} eq_dec (d: A) {l: list A} (Hn: NoDup l) {i: nat} (Hi: i < length l):
+  index eq_dec (nth i l d) l = i.
+Proof.
+  generalize dependent i. induction l as [| h t IH]; simpl; [lia|].
+  intros [| i'] Hi.
+  - destruct (eq_dec h h); auto. contradiction.
+  - inversion Hn as [| ? ? Hnotin Hn2]; subst; auto.
+    destruct (eq_dec (nth i' t d) h) as [Heq | Hneq]; auto. 2: f_equal; apply IH; auto; lia.
+    subst. exfalso. apply Hnotin. apply nth_In; lia.
+Qed.
 
 Section Proofs.
 
@@ -191,7 +516,6 @@ Context {gamma: context} (gamma_valid: valid_context gamma). (*old context*)
 Notation badnames := (idents_of_context gamma).
 
 Local Definition new_gamma := new_ctx new_constr_name keep_muts (idents_of_context gamma) noind gamma.
-Check new_gamma_gen_valid' .
 
 Variable (new_constrs_inj: forall (m1 m2 : mut_adt) (a1 a2 : alg_datatype),
 mut_in_ctx m1 gamma ->
@@ -217,14 +541,60 @@ Local Definition new_pf : pi_funpred new_gamma_valid pd new_pdf :=
   pf_new new_constr_name keep_muts noind gamma_valid pd pdf pf new_gamma_valid.
 Variable (vt: val_typevar).
 
-Check term_rep.
-Print rewriteT.
-
 (*TODO: why is it impossible to make something opaque*)
 Opaque n_str.
 Opaque under_str.
 
+(*TODO: is this useful above?*)
+Lemma simple_pat_match_constrs_uniq (b1: bool) {ps: list (pattern * gen_term b1)} 
+  (Hps: simple_pat_match (map fst ps)) {c tys1 tys2 pats1 pats2 t1 t2}
+  (Hinc1: In (Pconstr c tys1 pats1, t1) ps)
+  (Hinc2: In (Pconstr c tys2 pats2, t2) ps):
+  tys1 = tys2 /\ pats1 = pats2 /\ t1 = t2.
+Proof.
+  apply simple_pat_match_structure in Hps.
+  destruct Hps as [b [cs [Hnotnull [Hnodup Hmap]]]].
+  apply map_eq_app in Hmap.
+  destruct Hmap as [ps1 [ps2 [Hps [Hmap1 Hmap2]]]]. subst.
+  rewrite in_app_iff in Hinc1, Hinc2. destruct Hinc1 as [Hinc1 | Hinc1].
+  2: { apply (in_map fst) in Hinc1. rewrite Hmap2 in Hinc1; destruct b; [|contradiction].
+    destruct Hinc1 as [Heq | []]; discriminate. }
+  destruct Hinc2 as [Hinc2 | Hinc2].
+  2: { apply (in_map fst) in Hinc2. rewrite Hmap2 in Hinc2; destruct b; [|contradiction].
+    destruct Hinc2 as [Heq | []]; discriminate. }
+  (*Has to be better way*)
+  rewrite <- (combine_eq ps1) in Hinc1, Hinc2.
+  rewrite in_combine_iff in Hinc1, Hinc2; try solve_len.
+  rewrite map_length in Hinc1, Hinc2.
+  destruct Hinc1 as [i1 [Hi1 Heq1]]; destruct Hinc2 as [i2 [Hi2 Heq2]].
+  specialize (Heq1 Pwild (gen_d _)). specialize (Heq2 Pwild (gen_d _)).
+  inversion Heq1 as [Heq3]; subst; clear Heq1. inversion Heq2 as [Heq4]; subst; clear Heq2.
+  rewrite Hmap1 in Heq3, Heq4.
+  assert (Hlen: length ps1 = length cs). { apply (f_equal (fun x => length x)) in Hmap1. revert Hmap1.
+    solve_len. }
+  rewrite map_nth_inbound with (d2:=(id_fs, nil, nil)) in Heq3, Heq4; try lia.
+  inversion Heq3; inversion Heq4; subst; clear Heq3; clear Heq4.
+  assert (Hi12: i1 = i2). {
+    rewrite NoDup_nth with (d:=id_fs) in Hnodup. rewrite map_length in Hnodup.
+    specialize (Hnodup i1 i2 (ltac:(lia)) (ltac:(lia))).
+    rewrite !map_nth_inbound with (d2:=(id_fs, nil, nil)) in Hnodup by lia.
+    auto.
+  } subst. auto.
+Qed.
 
+Lemma fold_let_typed_inv {g} {l: list (term * vsymbol)} {t: term} {ty: vty}:
+  term_has_type g (fold_let Tlet l t) ty ->
+  Forall2 (term_has_type g) (map fst l) (map snd (map snd l)).
+Proof.
+  intros Hty. induction l as [| [t1 v1] tl IH]; simpl; auto.
+  simpl in Hty. inversion Hty; subst. constructor; auto.
+Qed.
+
+Check val_with_args.
+
+
+
+(*TODO: prove lemma for casting [val_with_args]*)
 
 Lemma rewrite_rep t f:
   (forall (ty: vty) (Hty1: term_has_type gamma t ty) 
@@ -315,7 +685,7 @@ Proof.
     reflexivity.
   - (*Tmatch*)
     intros tm ty1 ps IH1 IH2 ty Hty1. simpl. unfold is_true; rewrite !andb_true_iff.
-    intros [[Hsimp1 Hsimp2] Hsimppat] [[Hsimpexh Hex1] Hex2] Hty2 vv.
+    intros [[[Hsimp1 Hsimp2] Hsimppat] Hvardisj] [[Hsimpexh Hex1] Hex2] Hty2 vv.
     destruct (ty_match_inv Hty1) as [Hty1' [Hallpat Hallty]].
     (*Know the type is an ADT*)
     destruct (simple_pat_match_adt gamma_valid true ty Hsimppat Hty1) as 
@@ -364,4 +734,392 @@ Proof.
         inversion IH2'; subst. constructor; auto.
       - rewrite map_map. simpl. auto.
     } 
+    (*Main case*)
+    subst ty1. 
+    unfold get_constructors.
+    assert (Hts:find_ts_in_ctx gamma (adt_name a) = Some (m, a))
+      by (apply find_ts_in_ctx_iff; auto).
+    rewrite Hts.
+    set (tl := map _ (adt_constr_list a)) in *.
+    set (mp := (snd (mk_brs_tm _ _ _ _ _))) in *.
+    set (w:= (fst (mk_brs_tm _ _ _ _ _))) in *.
+    (*Get structure of pattern match*)
+    assert (Hsimp:=Hsimppat). apply simple_pat_match_structure in Hsimp.
+    destruct Hsimp as [b [cs [Hnotnull [Hnodup Hps]]]].
+    simpl_rep_full.
+    (*Find [semantic_constr] that we match on*)
+    set (d:= (term_rep gamma_valid pd pdf vt pf vv tm (vty_cons (adt_name a) args) (proj1' (ty_match_inv Hty1)))) in *.
+    destruct (find_semantic_constr gamma_valid pd pdf vt m_in a_in Hargslen d) as [c [[c_in al] Hsem]].
+    simpl in Hsem.
+    (*Will be useful*)
+    assert (Htmprops: forall p t, In (p, t) ps ->
+      pattern_has_type gamma p (vty_cons (adt_name a) args) /\
+      term_has_type gamma t ty /\
+      simple_pat p /\
+      term_simple_pats t /\
+      term_simple_exhaust gamma t /\
+      disj (tm_fv tm) (pat_fv p)).
+    {
+      intros p t Hinpt.
+      split_all.
+      - rewrite Forall_forall in Hallpat. specialize (Hallpat _ Hinpt). auto.
+      - rewrite Forall_forall in Hallty. specialize (Hallty _ Hinpt); auto.
+      - unfold is_true in Hallsimp; rewrite forallb_map, forallb_forall in Hallsimp.
+        specialize (Hallsimp _ Hinpt); auto.
+      - rewrite forallb_forall in Hsimp2; specialize (Hsimp2 _ Hinpt); auto.
+      - rewrite forallb_forall in Hex2; specialize (Hex2 _ Hinpt); auto.
+      - rewrite fold_is_true in Hvardisj.
+        rewrite match_vars_disj_equiv in Hvardisj. 
+        specialize (Hvardisj p). forward Hvardisj.
+        { rewrite in_map_iff. exists (p, t); auto. }
+        auto. 
+    }
+    destruct (get_single tl) as [[ tm1 Htl]| s].
+    + (*Case 1: only 1 constructor*)
+      destruct (adt_constr_list a)  as [| c1 [| c2 ctl]] eqn : Hconstrlist;
+      try solve[inversion Htl]. simpl.
+      simpl in tl.
+      (*Here, we know that c = c1, since only 1 constr*)
+      assert (c = c1). {
+        clear -c_in Hconstrlist.
+        apply in_bool_ne_In in c_in. unfold adt_constr_list in Hconstrlist. rewrite Hconstrlist in c_in.
+        destruct c_in as [Heq | []]; subst; auto.
+      }
+      subst c1.
+      (*Idea: case on whether constr c1 appears in ps or not.
+        If not, by [mk_brs_tm_snd_iff], must be none - use wild case
+        and show match falls through to wild case
+        If so, use NoDups (from [simple_pat_match_structure] to show unique,
+        show that each previous one in [match_rep] is None until we get to constr.
+        Then show it is in the map (TODO: will need to combine with later*)
+      destruct (existsb (fun p => is_this_constr p c) (map fst ps)) eqn : Hexconstr.
+      * apply existsb_exists in Hexconstr.
+        destruct Hexconstr as [p1 [Hinp1 Hp1]]. unfold is_this_constr in Hp1.
+        destruct p1 as [| f1 tys1 pats1 | | |]; try discriminate.
+        destruct (funsym_eq_dec _ _); subst; auto; [|discriminate].
+        rewrite in_map_iff in Hinp1. destruct Hinp1 as [[p2 t1] [Hp2 Hinpt]].
+        simpl in Hp2; subst p2. clear Hp1.
+        assert (Hmem: amap_mem funsym_eq_dec c mp). {
+          apply mk_brs_tm_snd_iff; auto. eexists; eexists; eauto. 
+        }
+        rewrite amap_mem_spec in Hmem.
+        destruct (amap_get funsym_eq_dec mp c) as [e|] eqn : Hget; [|discriminate]. clear Hmem.
+        simpl. assert (tm1 = e). { unfold tl in Htl. inversion Htl; subst; auto. }
+        subst e.
+        (*Now get info from map*)
+        apply mk_brs_tm_snd_get in Hget; [| solve[auto]].
+        destruct Hget as [tys2 [pats2 [t2 [Hinpt2 Htm1]]]]. subst tm1. clear Htl.
+        (*Use uniqueness*)
+        pose proof (simple_pat_match_constrs_uniq true Hsimppat Hinpt Hinpt2) as [Htys [Hpats Ht]].
+        subst tys2 pats2 t2. 
+        (*Get info about pattern and term*)
+        specialize (Htmprops _ _ Hinpt).
+        destruct Htmprops as  [Hpty [Htyt1 [Hsimpc [Hsimpt1 [Hext1 Hdisjp]]]]].
+        intros Hty2. simpl_rep_full.
+        (*We can simplify the RHS with [match_rep_simple_constr]*)
+        destruct (simpl_constr_get_vars Hsimpc) as [vars Hpats1]; subst pats1.
+        rewrite (match_rep_simple_constr gamma_valid m_in a_in c_in Hargslen pf vt vv true d 
+          (proj1' (proj2' (ty_match_inv Hty1))) (proj2' (proj2' (ty_match_inv Hty1))) Hsimppat Hinpt
+          Hsem).
+        simpl.
+        (*Note: both substitutions are iterated, so probably OK*)
+        (*Need lemma saying something like:
+          term_rep of fold_let Tlet l b is val_with_args pd vt vv (map fst l) (map (term_rep (map snd l))) b
+        (*NOTE: we need to know that these variables vs are not present in tm (and hence
+           rewriteT tm) - or else iterated substitution not same as ultiple substitution*)*)
+        (*So we do need to know: no variant in vars appears in tm (from pattern matching - these variables
+          are fresh*)
+        (*Have a bunch of preconditions for [fold_let_rep]*)
+        assert (Hty': term_has_type new_gamma (rewriteT keep_muts new_constr_name badnames gamma badvars t1) ty).
+        { unfold new_gamma, new_ctx. apply rewriteT_typed; auto. apply sublist_refl. }
+        set (l:=map2 _ _ _) in *.
+        assert (Htyall: Forall2 (term_has_type new_gamma) (map fst l) (map snd (map snd l))).
+        {
+          (*could prove directly but easier to prove from inversion*)
+          apply fold_let_typed_inv in Hty2. auto.
+        }
+        assert (Hnodupvars: NoDup vars).
+        { (*From typing*)
+          inversion Hpty; subst. rewrite NoDup_nth with (d:=vs_d).
+          intros i j Hi Hj Heq. clear -H10 Heq Hi Hj.
+          rewrite map_length in H10. specialize (H10 i j Pwild (nth i vars vs_d)).
+          destruct (Nat.eq_dec i j); subst; auto.
+          specialize (H10 Hi Hj n). exfalso; apply H10; clear H10.
+          rewrite !map_nth_inbound with (d2:=vs_d); auto. simpl.
+          split; left; auto.
+        }
+        assert (Hlen: length vars = length (get_proj_list badnames c)).
+        { unfold get_proj_list. rewrite projection_syms_length.
+          inversion Hpty; subst; auto. rewrite <- (map_length Pvar); auto.
+        }
+        assert (Hsnd: map snd l = vars). {
+          unfold l. clear -Hlen.
+          generalize dependent (get_proj_list badnames c).
+          induction vars as [|v1 tl1 IH]; simpl; intros [| hd2 tl2]; auto; try discriminate.
+          simpl; intros Hlen. f_equal; auto.
+        }
+        assert (Hnodupl: NoDup (map snd l)) by (rewrite Hsnd; auto).
+        assert (Hdisjl: forall (v : vsymbol) (t : term), In v (map snd l) -> In t (map fst l) -> ~ In v (tm_fv t)).
+        {
+          (*Follows from Hvardisj*)
+          simpl in Hdisjp.
+          rewrite Hsnd.
+          intros v' t' Hinv' Hint' Hinv2.
+          assert (Hint2: sublist (tm_fv t') (tm_fv tm)).
+          {
+            intros x Hinx.
+            revert Hint'. unfold l. rewrite map2_combine, map_map. (*TODO: what do we need?*) Search tm.
+            clear -Hlen Hinx gamma_valid Hty1' Hsimp1 Hex1.
+            generalize dependent (get_proj_list badnames c).
+            induction vars as [| v1 vtl IH]; intros [| h1 hs]; simpl; try discriminate; try contradiction.
+            intros Hlen. intros [Ht' | Hint']; auto.
+            2: apply IH in Hint'; auto. subst. simpl in Hinx.
+            (*need free variables of rewriteT from typing*)
+            simpl_set_small. destruct Hinx as [Hinx | []].
+            eapply (rewriteT_fv _ _ _ (sublist_refl _) gamma_valid) in Hinx; eauto.
+          }
+          apply Hint2 in Hinv2.
+          apply (Hdisjp v'); auto. split; auto. simpl_set. exists (Pvar v'); split; auto.
+          -  apply in_map; auto.
+          - simpl. auto.
+        }
+        (*Now finally we can use [fold_let_rep]*)
+        rewrite fold_let_rep with (Hty1:=Hty')(Htys:=Htyall); auto.
+        (*Use IH to eliminate rewrite*)
+        rewrite Forall_forall in IH2'. rewrite (IH2' _ Hinpt Htyt1).
+        simpl.
+        erewrite term_rep_irrel.
+        apply tm_change_vv.
+        intros x Hinx.
+        (*TODO: maybe move*)
+        assert (Htys1: tys1 = args). {
+          apply (constr_pattern_is_constr gamma_valid m_in a_in) in Hpty.
+          destruct Hpty; auto.
+        } subst tys1.
+        (*Now we need to prove the two arg_lists equal - use projection definition*)
+        assert (Heq: sym_sigma_args c (map (v_subst vt) args) = map (v_subst vt) (map snd (map snd l))).
+        { rewrite Hsnd. rewrite (constr_pattern_var_types m_in a_in c_in Hargslen Hpty).
+          apply sym_sigma_args_map. rewrite (adt_constr_params gamma_valid m_in a_in c_in); auto.
+        }
+        (*TODO: definitely want other lemma - prove arg lists correct by projection*)
+        assert (Hal: (terms_to_hlist new_gamma_valid pd new_pdf new_pf vt vv (map fst l) (map snd (map snd l)) Htyall) =
+          cast_arg_list Heq al).
+        {
+          (*Prove element by element*)
+          apply hlist_ext_eq with (d:=s_int)(d':=dom_int _).
+          rewrite !map_length. intros i Hi.
+          assert (Hi': i < Datatypes.length (map snd (map snd l))) by solve_len.
+          rewrite terms_to_hlist_hnth with (Hi:=Hi').
+          rewrite hnth_cast_arg_list.
+          (*Now we need to reason about nth of l and its rep - easiest to have only 1 cast*)
+          apply move_dom_cast.
+          generalize dependent (eq_trans (cast_nth_eq Heq i s_int) (eq_sym (tm_hlist_cast vt Hi'))).
+          generalize dependent (tm_hlist_ty Htyall Hi').
+          subst l.
+          (*TODO: see what we need*) clear -Hi Hlen m_in a_in c_in Hargslen new_constrs_inj Hsem IH1 Hsimp1 Hex1 Hty1'.
+          rewrite !map_map.
+          rewrite !map_nth_inbound with (d2:=(tm_d, vs_d)) by auto.
+          rewrite map2_length in Hi. rewrite map_length in Hi.
+          rewrite map2_nth with (d1:=Pwild) (d2:=id_fs); try solve_len.
+          rewrite map_nth_inbound with (d2:=vs_d); auto; try lia.
+          (*Finally, a reasonable goal*)
+          simpl.
+          intros Hty Heq.
+          simpl_rep_full.
+          (*Rewrite with projection interp*)
+          set (f:=(nth i (get_proj_list badnames c) id_fs)) in *.
+          assert (Hinf: In f (projection_syms badnames c)). {
+            eapply in_proj_syms. 2: reflexivity.
+            unfold get_proj_list in Hi. rewrite projection_syms_length in Hi. lia.
+          }
+          assert (Hargslen': length (map (v_subst vt) args) = length (m_params m)) by solve_len.
+          unfold cast_dom_vty. rewrite !dom_cast_compose.
+          apply move_dom_cast.
+          unfold funs_new_full.
+          (*Use proj interp*)
+          rewrite (funs_new_proj _  gamma_valid pd pdf pf _ 
+            new_constrs_inj m_in a_in c_in f Hinf (map (v_subst vt) args) _ Hargslen').
+          unfold proj_interp.
+          case_find_constr. case_find_constr. Check proj_args_eq.
+          destruct (proj_args_eq _ _ _ _ _ _ _ _ _ _ _) as [x Hx].
+          simpl. simpl in Hx.
+          destruct (find_constr_rep _ _ _ _ _ _ _ _ _ _ _) as [c1 Hc1]. simpl.
+          (*Idea: from [semantic_constr] and this info, can show c and c1 are equal*)
+          (*First, simplify in Hx - idea: s_args f is just ADT. This is very, very annoying
+            thanks to the dependent types*)
+          unfold fun_arg_list in Hx; simpl in Hx.
+                    revert Hx.
+          gen_dom_cast. gen_dom_cast.
+          (*A hack*)
+          do 3(match goal with |- context [@proj1' ?t ?x ?y] => generalize dependent (@proj1' t x y) end).
+          unfold sym_sigma_args in *. Check projection_syms_sigma_args.
+           match goal with | |- context [cast_arg_list ?Heq ?x] => generalize dependent Heq end. simpl.
+          rewrite (projection_syms_args _ Hinf).
+          simpl. intros Heq1 Hall1 _ Heq2. 
+          revert Hall1 Heq1 Heq2. (*generalize dependent (s_params_Nodup f).
+          rewrite (projection_syms_params _ Hinf).*)
+          simpl. intros Hall1 Heq1 Heq2 Heq3. rewrite cast_arg_list_cons.
+          (*Finally, something useful*)
+          intros Hx. apply (f_equal hlist_hd) in Hx. simpl in Hx.
+          rewrite !scast_scast in Hx.
+          apply scast_switch in Hx.
+          revert Hx.
+          match goal with |- context [scast ?H ?x] => generalize dependent H end.
+          intros Heq4 Hx.
+          (*Finally, we have x in terms of a cast of a [term_rep] - this is useful*)
+          (*Just need to handle types and IH*)
+          assert (Hsubstret: (ty_subst (s_params f) args (f_ret c)) = vty_cons (adt_name a) args).
+          { 
+            rewrite (projection_syms_params _ Hinf).
+            rewrite (adt_constr_subst_ret gamma_valid m_in a_in c_in); auto. 
+            rewrite (adt_constr_params gamma_valid m_in a_in c_in); auto.
+          }
+          generalize dependent (ty_subst (s_params f) args (f_ret c)). intros ty2 Hall1 Heq4 Hx Hty2; subst ty2.
+          rewrite IH1 with (Hty1:=Hty1') in Hx by auto.
+          (*Now, we prove that we again satisfy [semantic_constr] and hence we can use injectivity*)
+          destruct Hc1 as [[c1_in al2] Hx'].
+          assert (Hsem2: semantic_constr gamma_valid pd pdf vt m_in a_in c1_in Hargslen (scast (eq_sym Heq4) x) al2).
+          {
+            unfold semantic_constr. rewrite Hx'. unfold dom_cast. rewrite !scast_scast. apply scast_eq_uip' .
+            simpl. f_equal. apply UIP_dec, Nat.eq_dec.
+          } 
+          (*Now we know constrs and arg lists have to be equal*)
+          assert (Hxd: (scast (eq_sym Heq4) x) = d). {
+            rewrite Hx. rewrite scast_scast, eq_trans_sym_inv_r. simpl.
+            unfold d. apply term_rep_irrel.
+          }
+          rewrite Hxd in Hsem2.
+          assert (Hcs: c = c1). {
+            eapply (semantic_constr_inj_c gamma_valid gamma_valid m_in m_in a_in c_in c1_in); eauto.
+          }
+          subst c1.
+          assert (c1_in = c_in) by (apply bool_irrelevance); subst c1_in.
+          assert (al2 = al). {
+            eapply (semantic_constr_inj_al gamma_valid gamma_valid m_in m_in a_in c_in); eauto.
+          }
+          subst al2.
+          destruct (funsym_eq_dec c c); [|contradiction]. assert (e = eq_refl) by (apply UIP_dec, funsym_eq_dec).
+          subst e. simpl.
+          (*Now just prove index equal then done*)
+          gen_dom_cast. intros Heq5. unfold f. 
+          rewrite index_eq_nodup.
+          2: { eapply NoDup_map_inv. apply proj_names_nodup. }
+          2: { unfold get_proj_list in Hi. lia. }
+          intros Heq6. apply dom_cast_eq.
+        }
+        (*And finish up*)
+        rewrite Hal. symmetry; erewrite val_with_args_cast; try reflexivity; auto.
+      * (*2nd case: constr does not appear, then go to wild - START*)
+    +
+
+
+
+  clear -Hsnd. generalize dependent l. intros; subst.
+        unfold val_with_args.
+         
+        reflexivity.
+        
+        subst vars.
+        f_equal.
+
+
+        rewrite (IH1 _ Hty1' Hsimp1 Hex1 Hty').
+
+forall (ty : vty) (Hty1 : term_has_type gamma tm ty),
+      term_simple_pats tm ->
+      term_simple_exhaust gamma tm ->
+      forall
+        (Hty2 : term_has_type new_gamma (rewriteT keep_muts new_constr_name badnames gamma badvars tm)
+                  ty) (vv : val_vars pd vt),
+      term_rep new_gamma_valid pd new_pdf vt new_pf vv
+        (rewriteT keep_muts new_constr_name badnames gamma badvars tm) ty Hty2 =
+      term_rep gamma_valid pd pdf vt pf vv tm ty Hty1
+
+        2: { 
+
+ Unshelve.
+        rewrite fold_is_true in Hvardisj.
+        rewrite match_vars_disj_equiv in Hvardisj.
+        specialize (Hvardisj (Pconstr c tys1 (map Pvar vars))).
+        forward Hvardisj. { rewrite in_map_iff. eexists; split; [| apply Hinpt]; auto. }
+        simpl in Hvardisj.
+        (*Will need free variables of rewriteT, we proved before*)
+        Search tm_fv rewriteT.
+
+ rewrite in_map_iff; eexists; eauto. apply in_map.
+
+
+In (Pconstr c tys1 (map Pvar vars), t1) ps
+        
+        Search match_vars_disj.
+        assert (Hdisj: disj vars 
+
+Check fold_let.
+
+
+        Print val_with_args.
+        (*Possible challenge: *)
+        Check find_semantic_constr.
+        
+).
+        (*Let's just prove lemma: Suppose we have [simpl_pat_match (map fst ps)]
+          and suppose that (Pconstr c tys pats, t) is in ps.
+          Suppose that d is [semantic_constr] of c.
+          Then match_rep d ps = matches_row pats*)
+Check match_rep.
+Check semantic_constr.
+
+
+        Search (?l = ?l1 ++ ?x :: ?l2).
+
+in_split: forall [A : Type] (x : A) (l : list A), In x l -> exists l1 l2 : list A, l = l1 ++ x :: l2
+
+
+        Search match_rep' app.
+
+match_rep_app2:
+  forall {gamma : context} (gamma_valid : valid_context gamma) (b : bool) (ret_ty : gen_type b) 
+    (pd : pi_dom) (pdf : pi_dom_full gamma pd) (pf : pi_funpred gamma_valid pd pdf) (vt : val_typevar)
+    (v : val_vars pd vt) (ps1 ps2 : list (pattern * gen_term b)) (ty : vty)
+    (dom_t : domain (dom_aux pd) (v_subst vt ty))
+    (Hty1 : Forall (fun x : pattern * gen_term b => pattern_has_type gamma (fst x) ty) (ps1 ++ ps2))
+    (Hty2 : Forall (fun x : pattern * gen_term b => gen_typed gamma b (snd x) ret_ty) (ps1 ++ ps2)),
+  (forall (p : pattern * gen_term b) (Hp : pattern_has_type gamma (fst p) ty),
+   In p ps1 -> match_val_single gamma_valid pd pdf vt ty (fst p) Hp dom_t = None) ->
+  match_rep gamma_valid pd pdf vt v (term_rep gamma_valid pd pdf vt pf) (formula_rep gamma_valid pd pdf vt pf) b
+    ret_ty ty dom_t (ps1 ++ ps2) Hty1 Hty2 =
+  match_rep gamma_valid pd pdf vt v (term_rep gamma_valid pd pdf vt pf) (formula_rep gamma_valid pd pdf vt pf) b
+    ret_ty ty dom_t ps2 (Forall_app_snd Hty1) (Forall_app_snd Hty2)
+
+        Search In NoDup app.
+
+
+
+
+ by auto.
+        Search amap_get snd mk_brs_tm.
+
+mk_brs_tm_snd_get:
+  forall (badnames : list string) (rewriteT : term -> term) (args : list vty) (t1 : term)
+    (pats : list (pattern * term)) (c : funsym) (tm : term),
+  forallb simple_pat (map fst pats) ->
+  amap_get funsym_eq_dec (snd (mk_brs_tm badnames rewriteT args t1 pats)) c = Some tm ->
+  exists (tys : list vty) (vs : list pattern) (t2 : term),
+    In (Pconstr c tys vs, t2) pats /\
+    tm =
+    fold_let Tlet
+      (map2
+         (fun (p : pattern) (pj : funsym) =>
+          match p with
+          | Pvar v => (Tfun pj args [t1], v)
+          | _ => (tm_d, vs_d)
+          end) vs (get_proj_list badnames c)) (rewriteT t2)
+
+        2: { 
+
+
+      (*idea: look at pattern list
+      (*Case on c1:
+        1. If c1 is in map, then 
+      
     
